sha/HMAC_isPRF.v
@@ -124,15 +124,17 @@ Proof. intros.
   apply InBlocks_len; assumption.
 Qed.
 
-Lemma splitAndPad_1to1 b1 b2: splitAndPad_v b1 = splitAndPad_v b2 -> b1 = b2.
+Lemma splitAndPad_1to1 b1 b2 (B:splitAndPad_v b1 = splitAndPad_v b2)
+       (L1: NPeano.divide 8 (length b1))
+       (L2: NPeano.divide 8 (length b2)): b1 = b2.
 Proof. intros.
-  apply splitAndPad_v_eq_inverse in H.
-  unfold sha_splitandpad_blocks in H.
-  apply toBlocks_injective in H; try apply sha_splitandpad_inc_InBlocks.
-  unfold sha_splitandpad_inc in H.
-  apply bytesToBits_injective in H. 
-    apply pad_inc_injective in H.
-    apply (bitsToBytes_injective8 _ _ H). admit. admit. (*Hole: injectivity of bitsToBytes!!*)
+  apply splitAndPad_v_eq_inverse in B.
+  unfold sha_splitandpad_blocks in B.
+  apply toBlocks_injective in B; try apply sha_splitandpad_inc_InBlocks.
+  unfold sha_splitandpad_inc in B.
+  apply bytesToBits_injective in B. 
+    apply pad_inc_injective in B.
+    apply (bitsToBytes_injective8 _ _ B L1 L2).
   apply isbyteZ_pad_inc. eapply HMAC_spec_pad.HMAC_Pad.bitsToBytes_isbyteZ. reflexivity.
   apply isbyteZ_pad_inc. eapply HMAC_spec_pad.HMAC_Pad.bitsToBytes_isbyteZ. reflexivity.
 Qed.
@@ -169,58 +171,90 @@ Variable A : OracleComp Blist (Bvector c) bool. (*I seem to need this variable h
 (*Hypothesis*)
 Parameter A_wf : well_formed_oc A.*)
 
+Variable P : Blist -> Prop.
+Variable HP: forall m, P m -> NPeano.divide 8 (length m).
+
+Lemma wrappedSAP_1_1_local (msg1 msg2 : Message P):
+      wrappedSAP splitAndPad_v msg1 = wrappedSAP splitAndPad_v msg2 -> msg1 = msg2.
+Proof. apply wrappedSAP_1_1. intros.
+  apply HP in H0; apply HP in H1.
+  apply splitAndPad_1to1; trivial.
+Qed. 
+
+Definition msg_eqb (msg1 msg2:Message P): bool.
+destruct msg1 as [m1 M1].
+destruct msg2 as [m2 M2].
+apply (list_EqDec bool_EqDec). apply m1. apply m2.
+Defined.
+
+Lemma Message_eqdec: EqDec (Message P).
+apply (Build_EqDec msg_eqb). 
+intros; unfold msg_eqb. destruct x as [m1 M1]. destruct y as [m2 M2].
+destruct (eqb_leibniz m1 m2). 
+split; intros.
+  apply H in H1; clear H H0. apply Extensionality.exist_ext. trivial.
+  apply H0; clear H H0. apply EqdepFacts.eq_sig_fst in H1. trivial.
+Qed.
+
 (* Assume h is a tau-PRF against adversary (PRF_h_A h_star_pad A_GHMAC) *)
-(*Hypothesis*)
-Definition h_PRF (A : OracleComp Blist (Bvector c) bool) tau := 
+Definition h_PRF (A : OracleComp (Message P) (Bvector c) bool) tau := 
            isPRF ({ 0 , 1 }^c) ({ 0 , 1 }^c) h_v (Bvector_EqDec (b c p)) (Bvector_EqDec c) tau 
                          (PRF_h_A (h_star_pad h_v fpad_v) 
-                                  (HMAC_PRF.A_GHMAC p splitAndPad_v A)).
+                                  (HMAC_PRF.A_GHMAC p Message_eqdec (wrappedSAP splitAndPad_v) A)).
 
 (* We could make similar predicates for the other definitions, or just
 assume the inequalities*)
-Definition h_star_WCR (A : OracleComp Blist (Bvector c) bool) epsilon := 
+Definition h_star_WCR (A : OracleComp (Message P) (Bvector c) bool) epsilon := 
        cAU.Adv_WCR (list_EqDec (Bvector_EqDec (b c p)))
              (Bvector_EqDec (b c p)) (h_star_pad h_v fpad_v)
-       ({ 0 , 1 }^c) (au_F_A (A_GHMAC p splitAndPad_v A)) <= epsilon.
+       ({ 0 , 1 }^c) (au_F_A (A_GHMAC p Message_eqdec (wrappedSAP splitAndPad_v) A)) <= epsilon.
 
-Definition dual_h_RKA (A : OracleComp Blist (Bvector c) bool) sigma:=
+Definition dual_h_RKA (A : OracleComp (Message P) (Bvector c) bool) sigma:=
     RKA_Advantage _ _ _ ({ 0 , 1 }^b c p) ({ 0 , 1 }^c) (dual_f h_v) (BVxor (b c p))
-      (HMAC_RKA_A h_v iv_v fpad_v opad_v ipad_v (A_GHMAC p splitAndPad_v A)) <= sigma.
+      (HMAC_RKA_A h_v iv_v fpad_v opad_v ipad_v (A_GHMAC p Message_eqdec (wrappedSAP splitAndPad_v) A)) <= sigma.
 
 Theorem HMAC_isPRF A (A_wf : well_formed_oc A) tau epsilon sigma 
         (HH1: h_PRF A tau) (HH2: h_star_WCR A epsilon) (HH3: dual_h_RKA A sigma):
         isPRF (Rnd (b c p)) (Rnd c) 
-              (HMAC h_v iv_v splitAndPad_v
+              (HMAC h_v iv_v (wrappedSAP splitAndPad_v)
                               fpad_v opad_v ipad_v)
-              _ _ (tau + epsilon + sigma) A.
+              Message_eqdec _ (tau + epsilon + sigma) A.
 Proof. unfold isPRF.
-  specialize (HMAC_PRF h_v iv_v splitAndPad_v splitAndPad_1to1
+  specialize (HMAC_PRF h_v iv_v Message_eqdec (wrappedSAP splitAndPad_v) wrappedSAP_1_1_local
                               fpad_v opad_ne_ipad A_wf).
   intros.
   eapply leRat_trans. apply H. clear H. 
   unfold h_PRF, isPRF in HH1.
-  unfold HMAC_common_defs.b in *. unfold HMAC_spec.b in *. unfold b in *. unfold GHMAC_PRF.b in *. unfold GNMAC_PRF.b in *.  unfold HMAC_spec.b in *.
+  unfold HMAC_common_defs.b in *. unfold HMAC_spec.b in *. unfold b in *. 
+    unfold GHMAC_PRF.b in *. unfold GNMAC_PRF.b in *.  unfold HMAC_spec.b in *.
+  unfold HMAC_spec_abstract.c in *.
   remember (@PRF_Advantage (Bvector (c + p)) (Bvector c) (Bvector c) ({ 0 , 1 }^c)
         ({ 0 , 1 }^c) h_v (Bvector_EqDec (c + p)) (Bvector_EqDec c)
         (@PRF_h_A (c + p) c c (@h_star_pad c p h_v fpad_v)
-           (@A_GHMAC c p splitAndPad_v A))). clear Heqr.
+           (@A_GHMAC c p (Message P) Message_eqdec
+              (@wrappedSAP P splitAndPad_v) A))). clear Heqr.
   unfold h_star_WCR in HH2.
-  unfold HMAC_common_defs.b in *. unfold HMAC_spec.b in *. unfold b in *. unfold GHMAC_PRF.b in *. unfold GNMAC_PRF.b in *.  unfold HMAC_spec.b in *.
+  unfold HMAC_common_defs.b in *. unfold HMAC_spec.b in *. unfold b in *.
+    unfold GHMAC_PRF.b in *. unfold GNMAC_PRF.b in *.  unfold HMAC_spec.b in *.
+  unfold HMAC_spec_abstract.c in *.
   remember (@cAU.Adv_WCR (Bvector c) (list (Bvector (c + p))) (Bvector (c + p))
         (@list_EqDec (Bvector (c + p)) (Bvector_EqDec (c + p)))
         (Bvector_EqDec (c + p)) (@h_star_pad c p h_v fpad_v) ({ 0 , 1 }^c)
-        (@au_F_A (c + p) c (@A_GHMAC c p splitAndPad_v A))).
-  clear Heqr0.
+        (@au_F_A (c + p) c
+           (@A_GHMAC c p (Message P) Message_eqdec
+              (@wrappedSAP P splitAndPad_v) A))). clear Heqr0.
   unfold dual_h_RKA in HH3.
-  unfold HMAC_common_defs.b in *. unfold HMAC_spec.b in *. unfold b in *. unfold GHMAC_PRF.b in *. unfold GNMAC_PRF.b in *.  unfold HMAC_spec.b in *.
+  unfold HMAC_common_defs.b in *. unfold HMAC_spec.b in *. unfold b in *.
+    unfold GHMAC_PRF.b in *. unfold GNMAC_PRF.b in *.  unfold HMAC_spec.b in *.
+  unfold HMAC_spec_abstract.c in *.
   remember (@RKA_Advantage (Bvector (c + p)) (Bvector c) (Bvector c)
         (Bvector (c + p)) (Bvector_EqDec (c + p)) (Bvector_EqDec c)
         (Bvector_EqDec c) ({ 0 , 1 }^c + p) ({ 0 , 1 }^c)
         (@dual_f (Bvector c) (Bvector (c + p)) (Bvector c) h_v)
         (BVxor (c + p))
         (@HMAC_RKA_A c p h_v iv_v fpad_v opad_v ipad_v
-           (@A_GHMAC c p splitAndPad_v A)) ).
-  clear Heqr1.
+           (@A_GHMAC c p (Message P) Message_eqdec
+              (@wrappedSAP P splitAndPad_v) A))). clear Heqr1.
   rewrite ratAdd_comm. 
   apply ratAdd_leRat_compat; trivial. apply ratAdd_leRat_compat; trivial. (*What's the "omega" tactic for Rat?*)
 Qed.
@@ -281,4 +315,5 @@ Proof. unfold isPRF.
   rewrite ratAdd_comm. 
   apply ratAdd_leRat_compat; trivial. apply ratAdd_leRat_compat; trivial. (*What's the "omega" tactic for Rat?*)
 Qed.
-End HMAC_is_PRF. Runs out of memory*) 
+End HMAC_is_PRF. Runs out of memory*)
+  Print Assumptions HMAC_isPRF. 
